Test.thy
@@ -1,0 +1,40 @@
+theory Test      
+  imports Words Regular
+begin
+
+(* Trivial Word Equation *)
+lemma  "EX x. x = (of_list ''abc'')"
+  apply(auto)
+  done
+
+(* Word Equation constant RHS *)
+lemma  assumes s:"x = (of_list ''a'') \<and> y = (of_list ''c'')" shows "x * (of_list ''b'')  * y = (of_list ''abc'')"
+  apply(simp add: s)
+  done
+
+(* Word Equation with two patterns *)
+lemma  assumes s:"x = (of_list ''b'') \<and> y = (of_list ''c'')" shows "x * (of_list ''b'')  * y = x*x*y"
+  apply(simp add: s)
+  done
+
+
+(* Regular Memberships *)
+
+lemma  assumes s:"x = (of_list ''abc'')" shows "x \<in> (Const (of_list ''abc''))"
+  apply(simp add: s)
+  done
+
+lemma  assumes s:"x = (of_list ''abc'')" shows "x \<in> (Concat (Union (Const (of_list ''a''))(Const (of_list ''c'')))  (Const (of_list ''bc'')))"
+  apply(simp add: s)
+  done
+
+lemma  assumes s:"x = (of_list ''abbbbbc'')" shows "x \<in> (Concat (Const (of_list ''a'')) (Concat (Star (Const (of_list ''b''))) (Const (of_list ''c''))))"
+  apply(simp add: s)
+  done
+
+lemma  assumes s:"x = (of_list ''abdbbbbc'')" shows "\<not>x \<in> (Concat (Const (of_list ''a'')) (Concat (Star (Const (of_list ''b''))) (Const (of_list ''c''))))"
+  apply(simp add: s)
+  done
+
+
+end
